#Math 
## $\displaystyle \Gamma(z)=(z-1)! =\int_{0}^{\infty} t^{z-1}e^{-t} \, \mathrm{d}t$
* This is the analytic continuation of the factorial function
## $\displaystyle \Gamma(z+1)=z\Gamma(z)$
* Proven by [[integration by parts]]
* Like a factorial
## $\displaystyle \Gamma\left( \frac{1}{2} \right)=\sqrt{ \pi }$
* Can be shown by raw computation or by techniques in [[complex analysis]]
## $\displaystyle \Gamma\left( \frac{2n+1}{2} \right)=\sqrt{ \pi }\prod_{i = 1}^{n} \left(  \frac{2i-1}{2} \right)$
* Combines $\displaystyle \Gamma(z+1)=z\Gamma(z)$ with $\displaystyle \Gamma\left( \frac{1}{2} \right)=\sqrt{ \pi }$