#Math 
## $\displaystyle H_{n}(X)=(-1)^{n}e^{X^{2}}\frac{ \partial^{n}  }{ \partial X^{n} }e^{-X^{2}}$
* Used for solution of [[Quantum Harmonic Oscillator]]
* Expands to $\displaystyle n$th order polynomials due to cancellations of $\displaystyle e^{X^{2}}$ with $\displaystyle e^{-X^{2}}$
* Example:
* $\displaystyle H_{1}(X)=(-1)^{1}e^{X^{2}}\frac{ \partial  }{ \partial X }e^{-X^{2}}=-1\cdot e^{X^{2}}(-2Xe^{-X^{2}})=2X$
## $\displaystyle H(X)=\sum_{j = 0}^{\infty}a_{j}X^{j},a_{j+2}=\frac{2j-k+1}{(j+1)(j+2)}a_{j}$
* Power series representation of the above equation